Unordered_Resolution/Resolution_FOL/Completeness.thy
@@ -101,7 +101,7 @@ lemma complements_do_not_falsify':
   shows "False"
 proof (cases l\<^sub>1)
   case (Pos p ts)
-  let ?i1 = "nat_from_fatom (p, ts)"
+  let ?i1 = "nat_of_fatom (p, ts)"
 
   from assms have gr: "ground\<^sub>l l\<^sub>1" unfolding falsifies\<^sub>l_def by auto
   then have Neg: "l\<^sub>2 = Neg p ts" using comp Pos by (cases l\<^sub>2) auto
@@ -109,7 +109,7 @@ proof (cases l\<^sub>1)
   from falsif have "falsifies\<^sub>l G l\<^sub>1" using l1C1' by auto
   then have "G ! ?i1 = False" using l1C1' Pos unfolding falsifies\<^sub>l_def by (induction "Pos p ts") auto
   moreover
-  let ?i2 = "nat_from_fatom (get_atom l\<^sub>2)"
+  let ?i2 = "nat_of_fatom (get_atom l\<^sub>2)"
   from falsif have "falsifies\<^sub>l G l\<^sub>2" using l\<^sub>2C1' by auto
   then have "G ! ?i2 = (\<not>sign l\<^sub>2)" unfolding falsifies\<^sub>l_def by meson
   then have "G ! ?i1 = (\<not>sign l\<^sub>2)" using Pos Neg comp by simp
@@ -117,7 +117,7 @@ proof (cases l\<^sub>1)
   ultimately show ?thesis by auto
 next
   case (Neg p ts)
-  let ?i1 = "nat_from_fatom (p,ts)"
+  let ?i1 = "nat_of_fatom (p,ts)"
 
   from assms have gr: "ground\<^sub>l l\<^sub>1" unfolding falsifies\<^sub>l_def by auto
   then have Pos: "l\<^sub>2 = Pos p ts" using comp Neg by (cases l\<^sub>2) auto
@@ -125,7 +125,7 @@ next
   from falsif have "falsifies\<^sub>l G l\<^sub>1" using l1C1' by auto
   then have "G ! ?i1 = True" using l1C1' Neg unfolding falsifies\<^sub>l_def by (metis get_atom.simps(2) literal.disc(2)) 
   moreover
-  let ?i2 = "nat_from_fatom (get_atom l\<^sub>2)"
+  let ?i2 = "nat_of_fatom (get_atom l\<^sub>2)"
   from falsif have "falsifies\<^sub>l G l\<^sub>2" using l\<^sub>2C1' by auto
   then have "G ! ?i2 = (\<not>sign l\<^sub>2)" unfolding falsifies\<^sub>l_def by meson
   then have "G ! ?i1 = (\<not>sign l\<^sub>2)" using Pos Neg comp by simp
@@ -142,11 +142,11 @@ using assms complements_do_not_falsify' by blast
 
 lemma other_falsified:
   assumes C1'_p: "ground\<^sub>l\<^sub>s C\<^sub>1' \<and> falsifies\<^sub>g (B@[d]) C\<^sub>1'" 
-  assumes l_p: "l \<in> C\<^sub>1'" "nat_from_fatom (get_atom l) = length B"
+  assumes l_p: "l \<in> C\<^sub>1'" "nat_of_fatom (get_atom l) = length B"
   assumes other: "lo \<in> C\<^sub>1'" "lo \<noteq> l"
   shows "falsifies\<^sub>l B lo"
 proof -
-  let ?i = "nat_from_fatom (get_atom lo)"
+  let ?i = "nat_of_fatom (get_atom lo)"
   have ground_l\<^sub>2: "ground\<^sub>l l" using l_p C1'_p by auto
   -- {* They are, of course, also ground: *}
   have ground_lo: "ground\<^sub>l lo" using C1'_p other by auto
@@ -155,20 +155,20 @@ proof -
   then have loB\<^sub>2: "falsifies\<^sub>l (B@[d]) lo" using other by auto
   then have "?i < length (B @ [d])" unfolding falsifies\<^sub>l_def by meson
   -- {* And they have numbers in the range of @{term "B@[d]"}, i.e. less than @{term "length B + 1"}: *}
-  then have "nat_from_fatom (get_atom lo) < length B + 1" using undiag_diag_fatom by (cases lo) auto
+  then have "nat_of_fatom (get_atom lo) < length B + 1" using undiag_diag_fatom by (cases lo) auto
   moreover
   have l_lo: "l\<noteq>lo" using other by auto
   -- {* The are not the complement of @{term l }, since then the clause could not be falsified: *}
   have lc_lo: "lo \<noteq> l\<^sup>c" using C1'_p l_p other complements_do_not_falsify[of lo C\<^sub>1' l "(B@[d])"] by auto
   from l_lo lc_lo have "get_atom l \<noteq> get_atom lo" using sign_comp_atom by metis
-  then have "nat_from_fatom (get_atom lo) \<noteq> nat_from_fatom (get_atom l)" 
-    using nat_from_fatom_bij ground_lo ground_l\<^sub>2 ground\<^sub>l_ground_fatom 
+  then have "nat_of_fatom (get_atom lo) \<noteq> nat_of_fatom (get_atom l)" 
+    using nat_of_fatom_bij ground_lo ground_l\<^sub>2 ground\<^sub>l_ground_fatom 
     unfolding bij_betw_def inj_on_def by metis
   -- {* Therefore they have different numbers: *}
-  then have "nat_from_fatom (get_atom lo) \<noteq> length B" using l_p by auto
+  then have "nat_of_fatom (get_atom lo) \<noteq> length B" using l_p by auto
   ultimately 
   -- {* So their numbers are in the range of @{term B}: *}
-  have "nat_from_fatom (get_atom lo) < length B" by auto
+  have "nat_of_fatom (get_atom lo) < length B" by auto
   -- {* So we did not need the last index of @{term "B@[d]"} to falsify them, i.e. @{term B} suffices: *}
   then show "falsifies\<^sub>l B lo" using loB\<^sub>2 shorter_falsifies\<^sub>l by blast
 qed
@@ -233,7 +233,7 @@ text_raw {*}%EndSnippet*}
 
     -- {* @{term C\<^sub>1'} contains a literal @{term l\<^sub>1} that is falsified by @{term ?B\<^sub>1}, but not @{term B}: *}
     from C\<^sub>1'_p l_B obtain l\<^sub>1 where l\<^sub>1_p: "l\<^sub>1 \<in> C\<^sub>1' \<and> falsifies\<^sub>l (B@[True]) l\<^sub>1 \<and> \<not>(falsifies\<^sub>l B l\<^sub>1)" by auto
-    let ?i = "nat_from_fatom (get_atom l\<^sub>1)"
+    let ?i = "nat_of_fatom (get_atom l\<^sub>1)"
 
     -- {* @{term l\<^sub>1} is of course ground: *}
     have ground_l\<^sub>1: "ground\<^sub>l l\<^sub>1" using C\<^sub>1'_p l\<^sub>1_p by auto
@@ -247,7 +247,7 @@ text_raw {*}%EndSnippet*}
 
     -- {* @{term l\<^sub>1} is negative: *}
     from l\<^sub>1_sign_no have l\<^sub>1_sign: "sign l\<^sub>1 = False" by auto
-    from l\<^sub>1_sign_no have l\<^sub>1_no: "nat_from_fatom (get_atom l\<^sub>1) = length B" by auto
+    from l\<^sub>1_sign_no have l\<^sub>1_no: "nat_of_fatom (get_atom l\<^sub>1) = length B" by auto
 
     -- {* All the other literals in @{term C\<^sub>1'} must be falsified by B, since they are falsified by @{term ?B\<^sub>1}, but not @{term l\<^sub>1}. *}
     from C\<^sub>1'_p l\<^sub>1_no l\<^sub>1_p have B_C\<^sub>1'l\<^sub>1: "falsifies\<^sub>g B (C\<^sub>1' - {l\<^sub>1})" (* This should be a lemma *)
@@ -262,7 +262,7 @@ text_raw {*}%EndSnippet*}
     
     -- {* @{term C\<^sub>2'} contains a literal @{term l\<^sub>2} that is falsified by @{term ?B\<^sub>2}, but not B: *}
     from C\<^sub>2'_p l_B obtain l\<^sub>2 where l\<^sub>2_p: "l\<^sub>2 \<in> C\<^sub>2' \<and> falsifies\<^sub>l (B@[False]) l\<^sub>2 \<and> \<not>falsifies\<^sub>l B l\<^sub>2" by auto
-    let ?i = "nat_from_fatom (get_atom l\<^sub>2)"
+    let ?i = "nat_of_fatom (get_atom l\<^sub>2)"
 
     have ground_l\<^sub>2: "ground\<^sub>l l\<^sub>2" using C\<^sub>2'_p l\<^sub>2_p by auto
 
@@ -275,7 +275,7 @@ text_raw {*}%EndSnippet*}
 
     -- {* @{term l\<^sub>2} is negative: *}
     from l\<^sub>2_sign_no have l\<^sub>2_sign: "sign l\<^sub>2 = True" by auto
-    from l\<^sub>2_sign_no have l\<^sub>2_no: "nat_from_fatom (get_atom l\<^sub>2) = length B" by auto
+    from l\<^sub>2_sign_no have l\<^sub>2_no: "nat_of_fatom (get_atom l\<^sub>2) = length B" by auto
 
     -- {* All the other literals in @{term C\<^sub>2'} must be falsified by B, since they are falsified by 
           @{term ?B\<^sub>2}, but not @{term l\<^sub>2}. *}
@@ -287,7 +287,7 @@ text_raw {*}%EndSnippet*}
     have l\<^sub>2cisl\<^sub>1: "l\<^sub>2\<^sup>c = l\<^sub>1" (* Could perhaps be a lemma *)
       proof -
         from l\<^sub>1_no l\<^sub>2_no ground_l\<^sub>1 ground_l\<^sub>2 have "get_atom l\<^sub>1 = get_atom l\<^sub>2"
-              using nat_from_fatom_bij ground\<^sub>l_ground_fatom 
+              using nat_of_fatom_bij ground\<^sub>l_ground_fatom 
               unfolding bij_betw_def inj_on_def by metis
         then show "l\<^sub>2\<^sup>c = l\<^sub>1" using l\<^sub>1_sign l\<^sub>2_sign using sign_comp_atom by metis 
       qed
@@ -508,9 +508,9 @@ qed
   
 lemma infinite_hterms: "infinite (UNIV :: hterm set)"
 proof -
-  let ?diago = "\<lambda>n. HFun (string_from_nat n) []"
-  let ?undiago = "\<lambda>a. nat_from_string (case a of HFun f ts \<Rightarrow> f)"
-  have "\<forall>n. ?undiago (?diago n) = n" using nat_from_string_string_from_nat by auto
+  let ?diago = "\<lambda>n. HFun (string_of_nat n) []"
+  let ?undiago = "\<lambda>a. nat_of_string (case a of HFun f ts \<Rightarrow> f)"
+  have "\<forall>n. ?undiago (?diago n) = n" using nat_of_string_string_of_nat by auto
   moreover
   have "\<forall>n. ?diago n \<in> UNIV" by auto
   ultimately show "infinite (UNIV :: hterm set)" using infinity[of ?undiago ?diago UNIV] by simp
